refactor

LET/proof.v
@@ -1,136 +1,182 @@
-Require Import Bool ZArith Arith String List.
+Require Import Bool ZArith Arith List ClassicalEpsilon.
+Require Import Var Map.
 Set Implicit Arguments.
-
-Inductive expression : Set :=
-| Const : nat -> expression
-| Diff : expression -> expression -> expression
-| IsZero : expression -> expression
-| If : expression -> expression -> expression -> expression
-| Var : string -> expression
-| Let : string -> expression -> expression -> expression.
-
-Inductive expval : Set :=
-| Num : Z -> expval
-| Bool : bool -> expval.
-
-Definition environment := string -> option expval.
-Definition empty_env : environment := (fun _ => None).
-Definition extend_env (x : string) (v : expval) (env : environment) : environment :=
-  fun y => if string_dec x y then Some v else env y.
-
-Inductive value_of_rel : expression -> environment -> expval -> Prop :=
-| VConst :
-    forall num env,
-      value_of_rel (Const num) env (Num (Z.of_nat num))
-| VDiff :
-    forall exp1 exp2 num1 num2 env,
-      value_of_rel exp1 env (Num num1) ->
-      value_of_rel exp2 env (Num num2) ->
-      value_of_rel (Diff exp1 exp2) env (Num (num1 - num2))
-| VIsZero :
-    forall exp1 num1 env,
-      value_of_rel exp1 env (Num num1) ->
-      value_of_rel (IsZero exp1) env (Bool (Z.eqb num1 0))
-| VIfTrue :
-    forall exp1 exp2 exp3 val2 env,
-      value_of_rel exp1 env (Bool true) ->
-      value_of_rel exp2 env val2 ->
-      value_of_rel (If exp1 exp2 exp3) env val2
-| VIfFalse :
-    forall exp1 exp2 exp3 val3 env,
-      value_of_rel exp1 env (Bool false) ->
-      value_of_rel exp3 env val3 ->
-      value_of_rel (If exp1 exp2 exp3) env val3
-| VVar :
-    forall var env val,
-      env var = Some val -> value_of_rel (Var var) env val
-| VLet :
-    forall var exp1 body env val1 valb,
-      value_of_rel exp1 env val1 ->
-      value_of_rel body (extend_env var val1 env) valb ->
-      value_of_rel (Let var exp1 body) env valb.
 
 Notation "x <- e1 ; e2" :=
   (match e1 with
-   | None => None
    | Some x => e2
+   | None => None
    end)
     (right associativity, at level 60).
 
-Fixpoint value_of (exp : expression) (env : environment) : option expval :=
-  match exp with
-  | Const num => Some (Num (Z.of_nat num))
-  | Diff exp1 exp2 =>
-    val1 <- value_of exp1 env;
-      val2 <- value_of exp2 env;
-      match (val1, val2) with
-      | (Num num1, Num num2) => Some (Num (num1 - num2))
-      | _ => None
-      end
-  | IsZero exp1 =>
-    val1 <- value_of exp1 env;
-      match val1 with
-      | Num num1 => Some (Bool (Z.eqb num1 0))
-      | _ => None
-      end
-  | If exp1 exp2 exp3 =>
-    val1 <- value_of exp1 env;
-      match val1 with
-      | Bool true => value_of exp2 env
-      | Bool false => value_of exp3 env
-      | _ => None
-      end
-  | Var var => env var
-  | Let var exp1 body =>
-    val1 <- value_of exp1 env;
-      value_of body (extend_env var val1 env)
-  end.
+Module LetSpec.
+  Inductive expression : Set :=
+  | ExpConst : nat -> expression
+  | ExpDiff : expression -> expression -> expression
+  | ExpIsZero : expression -> expression
+  | ExpIf : expression -> expression -> expression -> expression
+  | ExpVar : var -> expression
+  | ExpLet : var -> expression -> expression -> expression.
 
-Hint Constructors value_of_rel.
+  Inductive expval : Set :=
+  | ValNum : Z -> expval
+  | ValBool : bool -> expval.
 
-Theorem value_of_soundness :
-  forall exp env val,
-    value_of exp env = Some val ->
-    value_of_rel exp env val.
-Proof.
-  induction exp; intros;
-    match goal with
-    | [ H : value_of _ _ = _ |- _ ] => simpl in H
-    end;
-    repeat (
-        try match goal with
-            | [ _ : context[match value_of ?EXP ?ENV with Some _ => _ | None => _ end] |- _ ] =>
-              destruct (value_of EXP ENV) eqn:?; try discriminate
-            | [ _ : context[match ?VAL with Num _ => _ | Bool _ => _ end] |- _ ] =>
-              destruct VAL; try discriminate
-            | [ _ : context[if ?B then _ else _] |- _ ] =>
-              destruct B
-            | [ H : Some _ = Some _ |- _ ] =>
-              inversion H; subst; clear H
-            end;
-        eauto).
-Qed.
+  Inductive value_of_rel : expression -> fmap var expval -> expval -> Prop :=
+  | VrelConst :
+      forall num env,
+        value_of_rel (ExpConst num) env (ValNum (Z.of_nat num))
+  | VrelDiff :
+      forall exp1 exp2 num1 num2 env,
+        value_of_rel exp1 env (ValNum num1) ->
+        value_of_rel exp2 env (ValNum num2) ->
+        value_of_rel (ExpDiff exp1 exp2) env (ValNum (num1 - num2))
+  | VrelIsZero :
+      forall exp1 num1 env,
+        value_of_rel exp1 env (ValNum num1) ->
+        value_of_rel (ExpIsZero exp1) env (ValBool (Z.eqb num1 0))
+  | VrelIfTrue :
+      forall exp1 exp2 exp3 val2 env,
+        value_of_rel exp1 env (ValBool true) ->
+        value_of_rel exp2 env val2 ->
+        value_of_rel (ExpIf exp1 exp2 exp3) env val2
+  | VrelIfFalse :
+      forall exp1 exp2 exp3 val3 env,
+        value_of_rel exp1 env (ValBool false) ->
+        value_of_rel exp3 env val3 ->
+        value_of_rel (ExpIf exp1 exp2 exp3) env val3
+  | VrelVar :
+      forall var env val,
+        env $? var = Some val -> value_of_rel (ExpVar var) env val
+  | VrelLet :
+      forall var exp1 body env val1 valb,
+        value_of_rel exp1 env val1 ->
+        value_of_rel body (env $+ (var, val1)) valb ->
+        value_of_rel (ExpLet var exp1 body) env valb.
 
-Theorem value_of_completeness :
-  forall exp env val,
-    value_of_rel exp env val ->
-    value_of exp env = Some val.
-Proof.
-  intros.
-  induction 0; simpl;
-    repeat (
-        try match goal with
-            | [ H : value_of ?EXP ?ENV = _ |- context[match value_of ?EXP ?ENV with Some _ => _ | None => _ end] ] =>
-              try (rewrite -> H; clear H)
-            end;
-        eauto).
-Qed.
+  Hint Constructors expression expval value_of_rel.
+End LetSpec.
 
-Theorem value_of_correctness :
-  forall exp env val,
-    value_of exp env = Some val <->
-    value_of_rel exp env val.
-Proof.
+Module LetImpl.
+  Export LetSpec.
+
+  Inductive environment : Set :=
+  | Empty : environment
+  | Extend : var -> expval -> environment -> environment.
+
+  Hint Constructors environment.
+
+  Definition empty_env : environment := Empty.
+
+  Fixpoint apply_env (env : environment) x :=
+    match env with
+    | Empty => None
+    | Extend x' v env' => if x ==v x' then Some v else apply_env env' x
+    end.
+
+  Definition extend_env (x : var) (v : expval) (env : environment) := Extend x v env.
+
+  Definition implemented env m := forall x, apply_env env x = m $? x.
+
+  Theorem implemented_empty : implemented empty_env $0.
+    unfold implemented, empty_env, apply_env.
+    intros.
+    autorewrite with core.
+    auto.
+  Qed.
+
+  Hint Resolve implemented_empty.
+
+  Theorem implemented_extend :
+    forall env m x v,
+      implemented env m ->
+      implemented (extend_env x v env) (m $+ (x, v)).
+  Proof.
+    unfold implemented, extend_env, apply_env.
+    intros.
+    destruct (x0 ==v x); autorewrite with core; auto.
+  Qed.
+
+  Hint Resolve implemented_extend.
+
+  Function value_of (exp : expression) (env : environment) : option expval :=
+    match exp with
+    | ExpConst num => Some (ValNum (Z.of_nat num))
+    | ExpDiff exp1 exp2 =>
+      val1 <- value_of exp1 env;
+        val2 <- value_of exp2 env;
+        match (val1, val2) with
+        | (ValNum num1, ValNum num2) => Some (ValNum (num1 - num2))
+        | _ => None
+        end
+    | ExpIsZero exp1 =>
+      val1 <- value_of exp1 env;
+        match val1 with
+        | ValNum num1 => Some (ValBool (Z.eqb num1 0))
+        | _ => None
+        end
+    | ExpIf exp1 exp2 exp3 =>
+      val1 <- value_of exp1 env;
+        match val1 with
+        | ValBool true => value_of exp2 env
+        | ValBool false => value_of exp3 env
+        | _ => None
+        end
+    | ExpVar var => apply_env env var
+    | ExpLet var exp1 body =>
+      val1 <- value_of exp1 env;
+        value_of body (extend_env var val1 env)
+    end.
+
+  Theorem value_of_soundness :
+    forall exp env val,
+      value_of exp env = Some val ->
+      forall m,
+      implemented env m ->
+      value_of_rel exp m val.
+  Proof.
+    induction exp; intros; rewrite value_of_equation in *;
+      repeat match goal with
+             | [ _ : context[match value_of ?EXP ?ENV with Some _ => _ | None => _ end] |- _ ] =>
+               destruct (value_of EXP ENV) eqn:?; try congruence
+             | [ _ : context[match ?VAL with ValNum _ => _ | ValBool _ => _ end] |- _ ] =>
+               destruct VAL; try congruence
+             | [ _ : context[if ?B then _ else _] |- _ ] =>
+               destruct B
+             | [ H : Some _ = Some _ |- _ ] =>
+               inversion H; clear H; subst
+             | [ H : implemented _ _ |- _ ] =>
+               unfold implemented in H; rewrite H in *
+             end;
+      eauto.
+  Qed.
+  
+  Theorem value_of_completeness :
+    forall exp m val,
+      value_of_rel exp m val ->
+      forall env,
+      implemented env m ->
+      value_of exp env = Some val.
+  Proof.
+    induction 1; intros; rewrite value_of_equation;
+      repeat match goal with
+             | [ H : forall _, implemented _ _ -> value_of _ _ = _ |- _ ] =>
+               rewrite H; clear H; subst; eauto
+             | [ H : implemented _ _ |- _ ] =>
+               unfold implemented in H; rewrite H in *
+             end;
+      eauto.
+  Qed.
+
   Hint Resolve value_of_soundness value_of_completeness.
-  intros; split; auto.
-Qed.
+  
+  Theorem value_of_correctness :
+    forall exp val,
+      value_of exp empty_env = Some val <->
+      value_of_rel exp $0 val.
+  Proof.
+    split; eauto.
+  Qed.
+End LetImpl.
+
+Export LetImpl.
